update lean 4 version

lean4/Crypto/Structure.lean
@@ -21,6 +21,7 @@ def AddToContext (lctx : LocalContext) (h : Name) (t : Expr) : MetaM (LocalConte
 
 -- #check Parser.Tactic.have
 structure FieldData where
+(decl : LocalDecl)
 (fvar : Expr)
 (type : Expr)
 (depends : NameSet)
@@ -32,49 +33,63 @@ instance : ToFormat NameSet :=
 ⟨λ x => fmt x.toList⟩
 
 instance : ToFormat FieldData :=
-⟨λ ⟨a, b, c, d⟩ => group (nest 1 (fmt "⟨"  ++ fmt a ++ fmt "," ++ line ++ fmt b ++ fmt "," ++ line
-++ fmt c ++ fmt "," ++ line ++ fmt d ++ fmt "⟩"))⟩
+⟨λ ⟨a, b, c, d, e⟩ => group (nest 1 (fmt "⟨"  ++ fmt a ++ fmt "," ++ line ++ fmt b ++ fmt "," ++ line
+++ fmt c ++ fmt "," ++ line ++ fmt d ++ fmt "," ++ line ++ fmt e ++ fmt "⟩"))⟩
+
+namespace FieldData
+
+def name (fields : FieldData) : Name :=
+fields.decl.userName.head!
+
+end FieldData
 
 namespace Meta
+
 def ppFieldData (x : FieldData) : MetaM Format :=
 do return group (nest 1 (fmt "⟨"  ++
+fmt x.name ++ fmt "," ++ line ++
 fmt (← ppExpr x.fvar) ++ fmt "," ++ line ++
 fmt (← ppExpr x.type) ++ fmt "," ++ line ++
 fmt (← x.depends.toList.mapM λ e => ppExpr (mkFVar e)) ++ fmt "," ++ line ++
 fmt x.isProp ++ fmt "⟩"))
 
-def AddFieldsToContext (mvarId : MVarId) (nm hnm : Name) (us : List Level) (args : Array Expr) :
-  MetaM (MVarId × Array FieldData) := do
+def AddFieldsToContext (mvarId : MVarId) (nm : Name) (us : List Level) (args : Array Expr) :
+  MetaM (MVarId × MVarId × Array FieldData) := do
   let e ← getEnv
   let d ← e.find? nm
   let tt ← isStructureLike e nm
   let eStr ← mkAppN (mkConst nm us) args
-  let (h, mvarId, m2) ← assertm mvarId hnm eStr
+  let (h, mvarId, m2) ← assertm mvarId `h eStr
   let l ← cases mvarId h
   let info := l.get! 0
   let mvarId := info.mvarId
   withMVarContext mvarId do
+  let lctx ← getLCtx
   let fieldExprs := info.fields
   let fields := fieldExprs.map Expr.fvarId!
+  let ldecls := fields.map λ e => lctx.fvarIdToDecl.find! e
   let axiom_fields ← fieldExprs.mapM isProof
   let types ← fieldExprs.mapM inferType
   let depends := types.map λ tp => tp.ListFvarIds
-  let fieldData := fieldExprs.zipWith4 FieldData.mk types depends axiom_fields
-  IO.println f!"field data: {← fieldData.mapM ppFieldData}"
-  return (mvarId, fieldData)
-
+  let fieldData := ldecls.zipWith5 FieldData.mk fieldExprs types depends axiom_fields
+  -- IO.println f!"field data: {← fieldData.mapM ppFieldData}"
+  return (mvarId, m2, fieldData)
+#print Array.foldr
 -- for testing
 def trivialMapping (lctx : LocalContext) (fields1 fields2 : Array FieldData) :
   MetaM $ Array Expr × Array Expr := do
-  let dataFields := fields1.filter $ λ info => !info.isProp
+  let dataFields := fields1.filter λ info => !info.isProp
   let map1 ← dataFields.map λ info => info.fvar
-  let map2 ← dataFields.map λ info => lctx.get! (info.fvar.fvarId!.updateSuffix $ λ s => "h2" ++ s) |>.toExpr
+  let map2 ← dataFields.map λ info => fields2.findSome! λ info' =>
+    if info.name == info'.name then some info'.fvar else none
+  -- let map2 := map2.map λ info? => info?.getD arbitrary
+  --(info.fvar.fvarId!.updateSuffix λ s => "h2" ++ s) |>.toExpr
   return (map1, map2)
 
 -- todo
 def allMappings (fields1 fields2 : Array FieldData) : MetaM $ List $ List (FVarId × Expr) := do
- let dataFields1 := fields1.filter $ λ info => !info.isProp
- let dataFields2 := fields2.filter $ λ info => !info.isProp
+ let dataFields1 := fields1.filter λ info => !info.isProp
+ let dataFields2 := fields2.filter λ info => !info.isProp
  throwError "todo"
 
 
@@ -86,67 +101,93 @@ def matchingAxioms (fields1 fields2 : Array FieldData) (map1 map2 : Array Expr) 
   let same ← propFields.filterM λ info => isIn (info.type.replaceFVars map1 map2) types2
   return same
 
-/-- The tactic we use to automatically prove axioms. -/
-def currentAutomation : MetaM Unit :=
-return () -- tidy >> (done <|> tactic.interactive.finish [] none)
+def mkSimpContext (simpOnly := false) : MetaM Simp.Context := do
+  return {
+    config      := {}
+    simpLemmas  := if simpOnly then {} else (← getSimpLemmas)
+    congrLemmas := (← getCongrLemmas)
+  }
 
--- /-- Tries to prove `e` in the local context, returns tt if successful. -/
--- def try_to_prove (e : Expr) : MetaM Bool := --retrieve $
--- do
---   assert `h e,
---   succeeds $ focus1 $ current_automation >> done
+/-- The tactic we use to automatically prove axioms. -/
+def currentAutomation (mvarId : MVarId) : MetaM Unit := do
+match (← simpTarget mvarId (← mkSimpContext false)) with -- does this work?
+| some x => return () --IO.println "failure!"
+| none => return ()  -- IO.println "success!"
+
+#print elabSimpConfig
+#print replaceMainGoal
+
+--return () -- tidy >> (done <|> tactic.interactive.finish [] none)
+
+/-- Tries to prove `e` in the local context, returns tt if successful. -/
+def tryToProve (mvarId : MVarId) (e : Expr) : MetaM Bool := withoutModifyingState do
+  let (fvar, mvarId, m2) ← assertm mvarId `h e
+  try
+    currentAutomation m2
+    -- IO.println s!"is assigned: {← isExprMVarAssigned m2}"
+    let some e ← getExprMVarAssignment? m2 | return false
+    let e ← instantiateMVars e
+    if (← e.hasExprMVar) then return false else return true
+  catch err =>
+    return false
+
 
 /-- Tests whether nm1 is a subclass of nm1. Currently the data fields must have the same Name for
 this tactic to work. -/
-def isSubclass (mvarId : MVarId) (nm1 nm2 : Name) (show_state := false) : MetaM MVarId := do
+def isSubclass (mvarId : MVarId) (nm1 nm2 : Name) (show_state := false) :
+  MetaM (MVarId × MVarId × MVarId) := do
   let u := mkLevelParam `u
   let (M, mvarId) ← asserti mvarId `M (mkSort (mkLevelSucc u)) (mkConst `PUnit [mkLevelSucc u])
-  let (mvarId, info1) ← AddFieldsToContext mvarId nm1 `h1 [u] #[mkFVar M]
-  let (mvarId, info2) ← AddFieldsToContext mvarId nm2 `h2 [u] #[mkFVar M]
+  let (mvarId, m1, fields1) ← AddFieldsToContext mvarId nm1 [u] #[mkFVar M]
+  let (mvarId, m2, fields2) ← AddFieldsToContext mvarId nm2 [u] #[mkFVar M]
   withMVarContext mvarId do
-  let (map1, map2) ← trivialMapping (← getLCtx) info1 info2
-  IO.println f!"map 1: {← map1.mapM Meta.ppExpr}"
-  IO.println f!"map 2: {← map2.mapM Meta.ppExpr}"
-  let n ← matchingAxioms info1 info2 map1 map2
-  let n_uniqs := n.map λ info => info.fvar.fvarId!
-  let todo := info1.filter λ info => info.isProp && !n_uniqs.contains info.fvar.fvarId!
-  (if todo.isEmpty then
-  IO.println s!"{nm1} is a trivial subclass of {nm2}: {nm2} has all the fields that {nm1} has." else do
-  -- trace $ todo.map $ λ info => info.fvar.local_pp_name,
-  -- let cannot_prove ← todo.filterM λ info => bnot <$> try_to_prove (info.type.instantiate_locals mapping),
-  let cannotProve := todo
-  -- trace $ cannot_prove.map $ λ info => info.fvar.local_pp_name,
-  if cannotProve.isEmpty then
-  IO.println s!"{nm1} is a subclass of {nm2}: {nm2} has all the data fields of {nm1}, and all the axioms of {nm1} can be proven from the axioms of {nm2}."
-  else
-  IO.println s!"Cannot prove the following axioms of {nm1} from the axioms of {nm2}:
-  {cannotProve.map $ λ info => info.fvar.fvarId!}.")
-  return mvarId
+  let (map1, map2) ← trivialMapping (← getLCtx) fields1 fields2
+  -- IO.println f!"map 1: {← map1.mapM Meta.ppExpr}"
+  -- IO.println f!"map 2: {← map2.mapM Meta.ppExpr}"
+  let matching ← matchingAxioms fields1 fields2 map1 map2
+  let matchingUniqs := matching.map λ info => info.fvar.fvarId!
+  let todo := fields1.filter λ info => info.isProp && !matchingUniqs.contains info.fvar.fvarId!
+  if todo.isEmpty then
+    IO.println s!"{nm1} is a trivial subclass of {nm2}: {nm2} has all the fields that {nm1} has."
+  else do
+    -- trace $ todo.map λ info => info.fvar.local_pp_name,
+    -- let cannot_prove ← todo.filterM λ info => bnot <$> try_to_prove (info.type.instantiate_locals mapping),
+    let cannotProve ← todo.filterM λ info =>
+      not <$> tryToProve mvarId (info.type.replaceFVars map1 map2)
+    -- trace $ cannot_prove.map λ info => info.fvar.local_pp_name,
+    if cannotProve.isEmpty then
+    IO.println s!"{nm1} is a subclass of {nm2}: {nm2} has all the data fields of {nm1}, and all the axioms of {nm1} can be proven from the axioms of {nm2}."
+    else
+    IO.println s!"Cannot prove the following axioms of {nm1} from the axioms of {nm2}:
+    {← cannotProve.mapM λ info : FieldData => ppExpr info.fvar}."
+  return (mvarId, m1, m2)
 
 end Meta
 open Meta
 
-def strucTacticM (mvarId : MVarId) : MetaM (MVarId × MVarId × Array FieldData) := do
-  let nm := `comm_monoid1
-  let e ← getEnv
-  let d ← e.find? nm
-  let tt ← isStructureLike e nm
-  let u := mkLevelParam `u
-  let (M, mvarId) ← asserti mvarId `M (mkSort (mkLevelSucc u)) (mkConst `PUnit [mkLevelSucc u])
-  let eStr ← mkAppN (mkConst nm [u]) #[mkFVar M]
-  let (h, mvarId, m2) ← assertm mvarId `h eStr
-  let l ← cases mvarId h
-  let info := l.get! 0
-  let mvarId := info.mvarId
-  withMVarContext mvarId do
-  let fieldExprs := info.fields
-  let fields := fieldExprs.map Expr.fvarId!
-  let axiom_fields ← fieldExprs.mapM isProof
-  let types ← fieldExprs.mapM inferType
-  let depends := types.map λ tp => tp.ListFvarIds
-  let fieldData := fieldExprs.zipWith4 FieldData.mk types depends axiom_fields
-  IO.println f!"field data: {← fieldData.mapM ppFieldData}"
-  return (mvarId, m2, fieldData)
+-- def strucTacticM (mvarId : MVarId) : MetaM (MVarId × MVarId × Array FieldData) := do
+--   let nm := `comm_monoid1
+--   let e ← getEnv
+--   let d ← e.find? nm
+--   let tt ← isStructureLike e nm
+--   let u := mkLevelParam `u
+--   let (M, mvarId) ← asserti mvarId `M (mkSort (mkLevelSucc u)) (mkConst `PUnit [mkLevelSucc u])
+--   let eStr ← mkAppN (mkConst nm [u]) #[mkFVar M]
+--   let (h, mvarId, m2) ← assertm mvarId `h eStr
+--   let l ← cases mvarId h
+--   let info := l.get! 0
+--   let mvarId := info.mvarId
+--   withMVarContext mvarId do
+--   let lctx ← getLCtx
+--   let fieldExprs := info.fields
+--   let fields := fieldExprs.map Expr.fvarId!
+--   let ldecls := fields.map λ e => lctx.fvarIdToDecl.find! e
+--   let axiom_fields ← fieldExprs.mapM isProof
+--   let types ← fieldExprs.mapM inferType
+--   let depends := types.map λ tp => tp.ListFvarIds
+--   let fieldData := ldecls.zipWith5 FieldData.mk fieldExprs types depends axiom_fields
+--   IO.println f!"field data: {← fieldData.mapM ppFieldData}"
+--   return (mvarId, m2, fieldData)
 
 
 syntax (name := assert) "assert " ident (" : " term) (" := " term)? : tactic
@@ -168,24 +209,24 @@ syntax (name := assert) "assert " ident (" : " term) (" := " term)? : tactic
         setGoals (m::l)
   | _ => throwUnsupportedSyntax
 
-syntax (name := struc) "struc" : tactic
-@[tactic «struc»] def evalStruc : Tactic := fun stx => do
-  match stx with
-  | `(tactic| struc) => withMainContext do
-    let mvarId ← getMainGoal
-    let (m1, m2, data) ← strucTacticM mvarId
-    let l ← getUnsolvedGoals
-    setGoals (m1::m2::l)
-  | _ => throwUnsupportedSyntax
+-- syntax (name := struc) "struc" : tactic
+-- @[tactic «struc»] def evalStruc : Tactic := fun stx => do
+--   match stx with
+--   | `(tactic| struc) => withMainContext do
+--     let mvarId ← getMainGoal
+--     let (m1, m2, data) ← strucTacticM mvarId
+--     let l ← getUnsolvedGoals
+--     setGoals (m1::m2::l)
+--   | _ => throwUnsupportedSyntax
 
 syntax (name := isSubclass) "isSubclass " ident ident : tactic
 @[tactic «isSubclass»] def evalIsSubclass : Tactic := fun stx => do
   match stx with
   | `(tactic| isSubclass $nm1 $nm2) => withMainContext do
     let mvarId ← getMainGoal
-    let mvarId ← Meta.isSubclass mvarId nm1.getId nm2.getId
+    let (mvarId, m1, m2) ← Meta.isSubclass mvarId nm1.getId nm2.getId
     let l ← getUnsolvedGoals
-    setGoals (mvarId::l)
+    setGoals (mvarId::m1::m2::l)
   | _ => throwUnsupportedSyntax
 
 /-! We define two notions of commutative monoids, the first is right-unital and the second is both left-unital and right-unital. -/
@@ -198,20 +239,28 @@ class comm_monoid1 (M : Type _) :=
 (mul_one : ∀ x, mul x one = x)
 
 class comm_monoid2 (M : Type _) :=
+(one : M)
 (mul : M → M → M)
+(mul_one : ∀ x, mul x one = x)
+(one_mul_one : mul one one = one)
+(one_mul : ∀ x, mul one x = x)
 (mul_assoc : ∀ x y z, mul (mul x y) z = mul x (mul y z))
 (mul_comm : ∀ x y, mul x y = mul y x)
-(one : M)
-(mul_one : ∀ x, mul x one = x)
-(one_mul : ∀ x, mul one x = x)
 
-example : Unit := by
-  struc
-  exact ()
+
+-- example : Unit := by
+--   struc
+--   exact ()
+--   admit
 
 example : Unit := by
   isSubclass comm_monoid1 comm_monoid2
+  isSubclass comm_monoid2 comm_monoid1
   exact ()
+  admit
+  admit
+  admit
+  admit
 
 -- #eval is_subclass `comm_monoid1 `comm_monoid2
 /- Output: comm_monoid1 is a trivial subclass of comm_monoid2: comm_monoid2 has all the fields that comm_monoid1 has. -/
